\documentclass{article}
% --- Modify margins --- %
\usepackage{geometry}
\geometry{a4paper,scale=0.8}
% --- Involved packages --- %
\usepackage{amssymb}
\usepackage{amsthm}
\usepackage{amsmath}
\usepackage{mathrsfs}
\usepackage{bbm}

% --- Title information --- %
\title{Math 733 - Fall 2020\\
        {\Large \textbf{Homework 3}}\\
        {\normalsize \textbf{Due: 10/11, 10pm}}
    }
\author{Zijie Zhang}
\date{\today}


% --- main --- %

\begin{document}
    \maketitle
    \begin{enumerate}
        % === Question 1 ===
        \item 
        \begin{enumerate}
        \item \begin{proof} 
            $$X\sim B(n,p) \Rightarrow P(X=k)=\binom{n}{k}p^k(1-p)^{n-k}$$
            $$Y\sim B(m,p) \Rightarrow P(X=k)=\binom{m}{k}p^k(1-p)^{m-k}$$
            Then \begin{align*}
                P(X+Y=k)&=\sum_{i=0}^k P(X=i, Y=k-i)\\
                &=\sum_{i=0}^k P(X=i)\cdot P(Y=k-i)\\
                &=\sum_{i=0}^k \binom{n}{i}p^i(1-p)^{n-i}
                    \cdot \binom{m}{k-i}p^{k-i}(1-p)^{m-k+i}\\
                &=p^k(1-p)^{m+n-k}\sum_{i=0}^k \binom{n}{i}\binom{m}{k-i}\\
                &=\binom{n+m}{k}p^k(1-p)^{m+n-k}
            \end{align*}
            Thus, $$X+Y \sim B(n+m,p)$$
        \end{proof}
        \item \begin{proof}
            $$X\sim \text{Poisson}(\lambda) \Rightarrow P(X=k)=\frac{\lambda^k}{k!}e^{-\lambda}$$
            $$Y\sim \text{Poisson}(\mu) \Rightarrow P(Y=k)=\frac{\mu^k}{k!}e^{-\mu}$$
            Then \begin{align*}
                P(X+Y=k)&=\sum_{i=0}^k P(X=i, Y=k-i)\\
                &=\sum_{i=0}^k P(X=i)\cdot P(Y=k-i)\\
                &=\sum_{i=0}^k \frac{\lambda^i}{i!}e^{-\lambda}
                    \cdot \frac{\mu^{k-i}}{(k-i)!}e^{-\mu}\\
                &=e^{-(\lambda+\mu)}\sum_{i=0}^k \frac{\lambda^i}{i!}\frac{\mu^{k-i}}{(k-i)!}\\
                &=\frac{(\lambda+\mu)^k}{k!}e^{-(\lambda+\mu)}
            \end{align*}
            Thus, $$X+Y \sim \text{Poisson}(\lambda+\mu)$$
        \end{proof}
        \end{enumerate}


        % === Question 2 ===
        \item \begin{enumerate}
            \item \begin{proof} 
                Let $h(x,y)=\mathbbm{1}_{\{xy\leqslant z\}}$, let $\mu,\nu$ be the probability measures with distributions $F_X$ and $F_Y$. Since for fixed $y>0$,
                $$\int{h(x,y)\mu(dx)}=\int{\mathbbm{1}_{(-\infty,z/y]}(x)\mu(dx)}=F_X(\frac{z}{y})$$
                
                So
                \begin{align*}
                    F_{XY}(z)=P(XY\leqslant z)&=\iint{\mathbbm{1}_{\{xy\leqslant z\}}\mu(dx)\nu(dy)}\\
                    &=\int F_X(\frac{z}{y})dF_Y(y)
                \end{align*}
            \end{proof}
            \item \begin{proof}
                Absolutely continuous means every set of measure zeros is probability zero. Consider
                $$P(XY)=P(X)P(Y)$$
                $$P(XY=x_1y_1)=P(X=x_1)P(Y=y_1)=0$$
                Then $XY$ is absolutely continuous with p.d.f
                $$f_{XY}=\int f_{X}\left(\frac{x}{t}\right)f_{Y}(t) \text{d}t$$
            \end{proof}
            \end{enumerate}


        % === Question 3 ===
        \item \begin{proof}
            \begin{align*}
                &\lim_{n\to\infty}P\left(|X_n+Y_n-(X+Y)|> \varepsilon\right)\\
                &\leqslant \lim_{n\to\infty}P\left(|X_n-X|>\frac{\varepsilon}{2}\right)+\lim_{n\to\infty}P\left(|Y_n-Y|>\frac{\varepsilon}{2}\right)\\
                &=0
            \end{align*}
            Since $X_n \overset{p}{\to} X$ and $Y_n \overset{p}{\to} Y$.
            So, $$X_n+Y_n \overset{p}{\to} X+Y$$

            \begin{align*}
                &\lim_{n\to\infty} P\left(|X_nY_n-XY|>\varepsilon\right)\\
                &=\lim_{n\to\infty} P\left(|(X_n-X)(Y_n-Y)+Y(X_n-X)+X(Y_n-Y)|>\varepsilon\right)\\
                &\leqslant\lim_{n\to\infty}P\left(|(X_n-X)(Y_n-Y)|>\frac{\varepsilon}{3}\right)+\lim_{n\to\infty}P\left(|Y(X_n-X)|>\frac{\varepsilon}{3}\right)+\lim_{n\to\infty}P\left(|X(Y_n-Y)|>\frac{\varepsilon}{3}\right)\\
                &=0
            \end{align*}
            $$X_n Y_n\overset{P}{\to}XY$$
        \end{proof}

        

        % === Question 4 ===
        \item \begin{proof}
            Consider $$x_i \sim U[0,1] \forall i \text{ and i.i.d}$$
            \begin{align*}
                &\lim_{n\to\infty}{\int_{0}^{1}{ \int_{0}^{1}{ \cdots \int_{0}^{1}}}} n\left(f\left(\frac{1}{n}(x_1+x_2+\cdots+x_n)\right)-f\left(\frac{1}{2}\right)\right)\text{d}x_1\text{d}x_2\cdots\text{d}x_n\\
                &=\lim_{n\to\infty}\mathbb{E}\left[n\left(f\left(\frac{1}{n}(x_1+x_2+\cdots+x_n)\right)-f\left(\frac{1}{2}\right)\right)\right]\\
                &=\lim_{n\to\infty} n\cdot\mathbb{E}\left[f\left(\frac{1}{n}(x_1+x_2+\cdots+x_n)\right)-f\left(\frac{1}{2}\right)\right]\\
                &f \text{ is continuous differentiable} \Leftrightarrow \mathbb{E}\left[f\left(\frac{x_1+x_2+\cdots+x_n}{n}\right)\right]=f\left(\mathbb{E}\left[\frac{x_1+x_2+\cdots+x_n}{n}\right]\right)\\
                &=\lim_{n\to\infty} n\cdot \left(f\left(\mathbb{E}\left[\frac{x_1+x_2+\cdots+x_n}{n}\right]\right)-f\left(\frac{1}{2}\right)\right)\\
                &\text{Since } \mathbb{E}\left[\frac{x_1+x_2+\cdots+x_n}{n}\right]=\mathbb{E}\left[x_1\right]=\int_{0}^1 t\text{d}t=\frac{1}{2}\\
                &\text{We have}\\
                &=\lim_{n\to\infty} n \cdot 0=0
            \end{align*}
        \end{proof}


        % === Question 5 ===
        \item \begin{enumerate}
            \item \begin{proof} 
                Let $$S_n=x_1+x_2+\cdots+x_n$$
                then $$\mathbb{E}[\mathbbm{1}_{\{S_k\leqslant x\}}]
                =P(S_k\leqslant x)
                =P(x_1+x_2+\cdots x_k<k)
                =F^{(k)}(x)$$
                Let $$N_x=\sum_{k=1}^{\infty}\mathbbm{1}_{\{S_k\leqslant x\}}$$
                It gives
                $$\mathbb{E}[N_x]=\sum_{n=1}^{\infty}\mathbb{E}[\mathbbm{1}_{\{S_n\leqslant x\}}]=\sum_{n=1}^{\infty}F^{(n)}(x)$$
            \end{proof}
            \item \begin{proof}
            Let $n=\lceil x \rceil$
               \begin{align*}
                   P(N_x=N)&=P(S_N \leqslant x <S_{N+1})\\
                   &\leqslant P(S_N \leqslant n)\\
                   &=\binom{N}{N-n}F^{(N-n)}(0)
               \end{align*}
               Consider the expectation,
               \begin{align*}
                   \mathbb{E}[N_x]&=\sum_{N=1}^{\infty}NP(N_x=N)\\
                   &\leqslant \sum_{N=1}^\infty N\binom{N}{N-n}F^{(N-n)}(0)\\
                   &\leqslant \sum_{N=1}^{\infty}N\binom{N}{n}F^{(N-n)}(0)\\
                   &<\infty
               \end{align*}
            \end{proof}
            \item \begin{proof}
                If$X_i$ are not integer, assume$X_i \in \mathbb{R}$.
                If $x_k < t$, let $x_k(t)=x_k$ else, let $x_k(t)=t$.
                Here we let $$N_x(t) = \sup_n{\{x_1(t)+x_2(t)+\cdots+x_n(t)\leqslant x\}}$$
                $$\mathbb{E}[N_x]\leqslant\mathbb{E}[N_x(t)]
                \leqslant \frac{\frac{x}{t}+1}{P(X\geqslant t)}<\infty$$
            \end{proof}
            \end{enumerate}


        % === Question 6 ===
        \item \begin{proof}
            Consider $X_1\sim \text{Cauchy(0,n)}$, $X_2\sim \text{Cauchy(0,1)}$ 
            \begin{align*}
                f_{X_1,X_2}(x_1,x_2)&=\frac{1}{n\pi^2\left(1+\left(\frac{x_1}{n}\right)^2\right)(1+x_2^2)}
            \end{align*}
            \begin{align*}
                f_{X_1+X_2,X_2}(x_1+x_2,x_2)&=\frac{1}{n\pi^2\left(1+\left(\frac{x_1+x_2}{n}\right)^2\right)(1+x_2^2)}
            \end{align*}
            \begin{align*}
                f_{X_1+X_2}(x_1+x_2)&=\int f_{X_1+X_2,X_2}(x_1+x_2,x_2) \text{d}x_2\\
                &=\int\frac{1}{n\pi^2\left(1+\left(\frac{x_1+x_2}{n}\right)^2\right)(1+x_2^2)}\\
                &=\int\frac{n}{\pi^2\left(n^2+\left(x_1+x_2\right)^2\right)(1+x_2^2)}\\
                &=\frac{1}{(n+1)\pi\left(1+\left(\frac{X_1+X_2}{n+1}\right)\right)}
            \end{align*}
            This means Cauchy distribution is additive.
            \begin{align*}
                S_n&=X_1+X_2+\cdots+X_n\sim\text{Cauchy}(0,n)\\
                P(S_n<x)&=\frac{1}{\pi}\arctan(\frac{x}{n})+\frac{1}{2}\\
                P(S_n<nx) &=\frac{1}{\pi}\arctan(x)+\frac{1}{2}\\
                &=P(X_1<x)
            \end{align*}
            So, $$\frac{S_n}{n}\sim X_1$$
            Which means
            $$\frac{S_n}{c_n}=\frac{S_n}{n}\frac{n}{c_n}\sim X_1\frac{n}{c_n}$$
            For all $x$,
            $$\lim_{n\to+\infty}\frac{S_n(x)}{c_n}=\lim_{n\to+\infty}\frac{S_n(x)}{n}\frac{n}{c_n}=0$$
            So, $$\frac{S_n}{c_n}\to 0 \Rightarrow \frac{S_n}{c_n}\overset{P}{\to}0$$
        \end{proof}
    
    \end{enumerate}
\end{document}